src/traversal/TraversalConfig.v
@@ -735,7 +735,7 @@ Section Properties.
   Proof using WF TCCOH.
     rewrite (dom_l WF.(wf_rfeD)).
     arewrite (rfe ⊆ ar).
-    arewrite (ppo ⊆ ar).
+    rewrite ppo_in_ar.
     sin_rewrite ar_ar_in_ar_ct.
       by apply ar_ct_I_in_I.
   Qed.
@@ -755,7 +755,7 @@ Section Properties.
     arewrite (rfe ⊆ ar).
     arewrite (detour ⊆ ar).
     relsf.
-    arewrite (ppo ⊆ ar).
+    rewrite ppo_in_ar, !seqA.
     sin_rewrite ar_ar_in_ar_ct.
     apply dom_ar_ct_issuable.
   Qed.
@@ -823,11 +823,11 @@ Section Properties.
   
   Lemma rf_rmw_issued_rfi_rmw_issued : 
     (rf ⨾ rmw)＊ ⨾ ⦗issued T⦘ ⊆ (rfi ⨾ rmw)＊ ⨾ ⦗issued T⦘ ⨾ (rf ⨾ rmw)＊.
-  Proof using WF TCCOH.
+  Proof using WF TCCOH IMMCON.
     assert (transitive sb) as SBT by apply sb_trans.
     eapply rt_ind_left with (P:= fun r => r ⨾ ⦗issued T⦘).
     { by eauto with hahn. }
-    basic_solver 12.
+    { basic_solver 12. }
     intros k H; rewrite !seqA.
     sin_rewrite H.
     rewrite rfi_union_rfe at 1; relsf; unionL.
@@ -837,20 +837,16 @@ Section Properties.
     arewrite (rfe ⨾ rmw ⨾ (rfi ⨾ rmw)＊ ⨾ ⦗issued T⦘ ⊆
                   ⦗issued T⦘ ⨾ rfe ⨾ rmw ⨾ (rfi ⨾ rmw)＊ ⨾ ⦗issued T⦘).
     { apply dom_rel_helper.
-      rewrite (rmw_in_sb WF) at 2; arewrite (rfi ⊆ sb) at 1.
-      sin_rewrite sb_sb.
-      rewrite (dom_l (wf_rmwD WF)) at 1; rewrite !seqA.
-      rewrite WF.(rmw_in_sb).
-      arewrite (sb ⨾ sb＊ ⊆ sb⁺).
-      rewrite ct_of_trans; auto.
-      rewrite (dom_l WF.(wf_rfeD)); rewrite !seqA.
-      arewrite (rfe ⊆ ar).
-      arewrite (⦗issued T⦘ ⊆ ⦗W⦘ ⨾ ⦗issued T⦘).
-      { rewrite <- seq_eqvK at 1. by rewrite issuedW at 1. }
-      sin_rewrite R_ex_sb_in_ppo; auto.
-      rewrite ppo_in_ar with (sc:=sc).
-      sin_rewrite ar_ar_in_ar_ct.
-        by apply ar_ct_I_in_I. }
+      arewrite (rmw ⨾ (rfi ⨾ rmw)＊ ⊆ ar^*).
+      { arewrite (rfi ⊆ rf).
+        rewrite WF.(rmw_in_ppo) at 1. rewrite ppo_in_ar.
+        rewrite rtE at 1. rewrite seq_union_r, seq_id_r.
+        apply inclusion_union_l.
+        { rewrite ct_step at 1. apply inclusion_t_rt. }
+        rewrite ar_rfrmw_ct_in_ar_ct; auto. apply inclusion_t_rt. }
+      rewrite (dom_l WF.(wf_rfeD)), !seqA.
+      arewrite (rfe ⊆ ar) at 1.
+      seq_rewrite <- ct_begin. by apply ar_ct_I_in_I. }
     arewrite (rfe ⨾ rmw ⊆ rf ⨾ rmw).
     arewrite (rfi ⊆ rf).
     arewrite (rf ⨾ rmw ⨾ (rf ⨾ rmw)＊ ⊆ (rf ⨾ rmw)⁺).
@@ -878,7 +874,7 @@ Section Properties.
       arewrite (ar ⊆ ar ∪ rf ⨾ rmw) at 1.
       basic_solver 10. }
     rewrite WF.(rmw_in_ppo).
-    arewrite (ppo ⊆ ar).
+    rewrite ppo_in_ar.
     rewrite (dom_l WF.(wf_rfeD)), !seqA.
     arewrite (rfe ⊆ ar).
     sin_rewrite ar_ar_in_ar_ct.
@@ -1015,7 +1011,7 @@ Section Properties.
 
   Lemma dom_release_issued :
     dom_rel (release ⨾ ⦗ issued T ⦘) ⊆₁ covered T.
-  Proof using WF TCCOH RELCOV.
+  Proof using WF TCCOH RELCOV IMMCON.
     unfold imm_s_hb.release, imm_s_hb.rs.
     rewrite !seqA.
     sin_rewrite rf_rmw_issued_rfi_rmw_issued.
@@ -1034,14 +1030,14 @@ Section Properties.
 
   Lemma release_issued :
     release ⨾ ⦗ issued T ⦘ ⊆ ⦗covered T⦘ ⨾ release.
-  Proof using WF TCCOH RELCOV.
+  Proof using WF TCCOH RELCOV IMMCON.
     seq_rewrite (dom_rel_helper dom_release_issued).
     basic_solver.
   Qed.
 
   Lemma dom_release_rf_coverable :
     dom_rel (release ⨾ rf ⨾ ⦗ coverable T ⦘) ⊆₁ covered T.
-  Proof using WF TCCOH RELCOV.
+  Proof using WF TCCOH RELCOV IMMCON.
     generalize dom_release_issued.
     generalize dom_rf_coverable.
     basic_solver 21.
@@ -1049,14 +1045,14 @@ Section Properties.
 
   Lemma release_rf_coverable :
     release ⨾ rf ⨾ ⦗ coverable T ⦘ ⊆ ⦗ covered T ⦘ ⨾ release ⨾ rf.
-  Proof using WF TCCOH RELCOV.
+  Proof using WF TCCOH RELCOV IMMCON.
     seq_rewrite (dom_rel_helper dom_release_rf_coverable).
     basic_solver.
   Qed.
 
   Lemma release_rf_covered :
     release ⨾ rf ⨾ ⦗ covered T ⦘ ⊆ ⦗ covered T ⦘ ⨾ release ⨾ rf.
-  Proof using WF TCCOH RELCOV.
+  Proof using WF TCCOH RELCOV IMMCON.
     rewrite covered_in_coverable at 1.
       by apply release_rf_coverable.
   Qed.
@@ -1082,7 +1078,7 @@ Section Properties.
 
   Lemma dom_sw_coverable :
     dom_rel (sw ⨾ ⦗ coverable T ⦘) ⊆₁ covered T.
-  Proof using WF TCCOH RELCOV.
+  Proof using WF TCCOH RELCOV IMMCON.
     unfold imm_s_hb.sw.
     generalize dom_sb_coverable.
     generalize dom_release_rf_coverable.
@@ -1091,19 +1087,19 @@ Section Properties.
   Qed.
 
   Lemma sw_coverable : sw ⨾ ⦗ coverable T ⦘ ⊆ ⦗covered T⦘ ⨾ sw.
-  Proof using WF TCCOH RELCOV.
+  Proof using WF TCCOH RELCOV IMMCON.
     seq_rewrite (dom_rel_helper dom_sw_coverable).
     basic_solver.
   Qed.
 
   Lemma sw_covered : sw ⨾ ⦗ covered T ⦘ ⊆ ⦗covered T⦘ ⨾ sw.
-  Proof using WF TCCOH RELCOV.
+  Proof using WF TCCOH RELCOV IMMCON.
     rewrite covered_in_coverable at 1.
       by apply sw_coverable.
   Qed.
 
   Lemma hb_coverable : hb ⨾ ⦗ coverable T ⦘ ⊆ ⦗covered T⦘ ⨾ hb.
-  Proof using WF TCCOH RELCOV.
+  Proof using WF TCCOH RELCOV IMMCON.
     unfold imm_s_hb.hb.
     assert (A: (sb ∪ sw) ⨾ ⦗coverable T⦘ ⊆ ⦗covered T⦘ ⨾ (sb ∪ sw)⁺).
     { relsf.
@@ -1140,13 +1136,13 @@ Qed.
 
   Lemma dom_hb_coverable :
     dom_rel (hb ⨾ ⦗ coverable T ⦘) ⊆₁ covered T.
-  Proof using WF TCCOH RELCOV.
+  Proof using WF TCCOH RELCOV IMMCON.
     rewrite hb_coverable; basic_solver 10.
   Qed.
 
   Lemma hb_covered :
     hb ⨾ ⦗ covered T ⦘ ⊆ ⦗covered T⦘ ⨾ hb.
-  Proof using WF TCCOH RELCOV.
+  Proof using WF TCCOH RELCOV IMMCON.
     rewrite covered_in_coverable at 1.
       by apply hb_coverable.
   Qed.
@@ -1296,7 +1292,7 @@ Qed.
 
   Lemma S_tm_coverable l :
     S_tm l (coverable T) ⊆₁ issued T.
-  Proof using WF TCCOH RELCOV.
+  Proof using WF TCCOH RELCOV IMMCON.
     unfold CombRelations.S_tm, CombRelations.S_tmr.
     generalize dom_hb_coverable.
     generalize w_coverable_issued.
@@ -1308,7 +1304,7 @@ Qed.
 
   Lemma S_tm_covered l:
     S_tm l (covered T) ⊆₁ issued T.
-  Proof using WF TCCOH RELCOV.
+  Proof using WF TCCOH RELCOV IMMCON.
     rewrite covered_in_coverable at 1.
       by apply S_tm_coverable.
   Qed.
@@ -1338,155 +1334,44 @@ Notation "'I'" := (issued  T).
 
 Lemma sw_in_Csw_sb :
   sw ⨾ ⦗C ∪₁ dom_rel (sb^? ⨾ ⦗ I ⦘)⦘ ⊆ ⦗ C ⦘ ⨾ sw ∪ sb.
-Proof using WF TCCOH RELCOV.
-  assert (forall (s : actid -> Prop), s ∪₁ set_compl s ≡₁ fun _ => True) as AA.
-  { split; [basic_solver|].
-    unfolder. ins. apply classic. }
+Proof using WF TCCOH RELCOV IMMCON.
   rewrite !id_union. rewrite seq_union_r. 
   unionL.
   { rewrite sw_covered; eauto. basic_solver. }
+  assert (forall (s : actid -> Prop), s ∪₁ set_compl s ≡₁ fun _ => True) as AA.
+  { split; [basic_solver|].
+    unfolder. ins. apply classic. }
   arewrite (sw ⊆ ⦗ C ∪₁ set_compl C ⦘ ⨾ sw) at 1.
   { rewrite AA. by rewrite seq_id_l. }
-  rewrite id_union. relsf.
+  rewrite id_union, !seq_union_l.
   apply union_mori; [basic_solver|].
-  unfold imm_s_hb.sw.
-  arewrite ((sb ⨾ ⦗F⦘)^? ⊆ sb ⨾ ⦗F⦘ ∪ ⦗ fun _ => True ⦘) by basic_solver.
+  rewrite (dom_r WF.(wf_swD)).
+  rewrite sw_in_ar0; auto.
+  remember (⦗Rel⦘ ⨾ (⦗F⦘ ⨾ sb)^? ⨾ ⦗W⦘ ⨾ (sb ∩ same_loc)^? ⨾ ⦗W⦘ ⨾ (rfe ∪ ar_int G)⁺) as ax.
   rewrite !seq_union_l, !seq_union_r.
-  unionL.
-  { rewrite !seqA.
-    seq_rewrite <- !id_inter. rewrite <- !set_interA.
-    arewrite (sb ⨾ ⦗F ∩₁ Acq ∩₁ dom_rel (sb^? ⨾ ⦗I⦘)⦘ ⊆
-              ⦗ C ⦘ ⨾ sb ⨾ ⦗F ∩₁ Acq ∩₁ dom_rel (sb^? ⨾ ⦗I⦘)⦘).
-    { unfolder. ins. desf; splits; auto.
-      2,4: by do 2 eexists; splits; eauto.
-      2: eapply dom_sb_covered.
-      2: eexists; apply seq_eqv_r; split; eauto.
-      all: match goal with H : I _ |- _ => apply TCCOH in H; apply H end.
-      all: eexists; apply seq_eqv_r; split; eauto.
-      { apply sb_to_f_in_fwbob. apply seq_eqv_r. split; [|split]; auto.
-        mode_solver. }
-      apply sb_from_f_in_fwbob. apply seq_eqv_l. split; [split|]; auto.
-      mode_solver. }
-    sin_rewrite release_rf_covered; eauto.
+  unionL; [|basic_solver].
+  subst ax. rewrite !seqA.
+  arewrite ((sb ∩ same_loc)^? ⨾ ⦗W⦘ ⊆ (sb ∩ same_loc)^? ⨾ ⦗W⦘ ⨾ ⦗W⦘) by basic_solver. 
+  arewrite (⦗Rel⦘ ⨾ (⦗F⦘ ⨾ sb)^? ⨾ ⦗W⦘ ⨾ (sb ∩ same_loc)^? ⨾ ⦗W⦘ ⊆ release).
+  { unfold imm_s_hb.release, imm_s_hb.rs. by rewrite <- inclusion_id_rt, seq_id_r. }
+  enough (dom_rel (⦗W⦘ ⨾ (rfe ∪ ar_int G)⁺ ⨾ ⦗FR ∩₁ Acq⦘ ⨾ ⦗dom_rel (sb^? ⨾ ⦗I⦘)⦘) ⊆₁ I) as BB.
+  { rewrite (dom_rel_helper BB).
+    seq_rewrite (dom_rel_helper dom_release_issued).
     basic_solver. }
-  rewrite seq_id_l.
-  arewrite (rf ⊆ ⦗ I ∪₁ set_compl I⦘ ⨾ rf).
-  { rewrite AA. basic_solver. }
-  rewrite id_union. relsf.
-  unionL.
-  { sin_rewrite release_issued; eauto. basic_solver. }
-  rewrite rfi_union_rfe. relsf.
-  unionL.
-  2: { arewrite (⦗set_compl I⦘ ⨾ rfe ⨾ ⦗Acq⦘ ⨾ ⦗dom_rel (sb^? ⨾ ⦗I⦘)⦘ ⊆ ∅₂).
-       2: basic_solver.
-       seq_rewrite <- !id_inter.
-       unfolder. ins. desf.
-       { match goal with H : I _ |- _ => apply issuedW in H end.
-         match goal with H : rfe _ _ |- _ =>
-                         apply wf_rfeD in H; auto; (destruct_seq H as [XX YY])
-         end.
-         type_solver. }
-       match goal with H : ~ (I _) |- _ => apply H end.
-       eapply dom_rfe_acq_sb_issued; eauto.
-       eexists. eexists. split; eauto.
-       apply seq_eqv_l. split; [split|]; auto.
-       2: { apply seq_eqv_r. split; eauto. }
-       match goal with H : rfe _ _ |- _ =>
-                       apply wf_rfeD in H; auto; (destruct_seq H as [XX YY]); auto
-       end. }
-  unfold imm_s_hb.release, rs.
-  arewrite
-    (⦗set_compl C⦘ ⨾ (⦗Rel⦘ ⨾ (⦗F⦘ ⨾ sb)^? ⨾ ⦗W⦘ ⨾ (sb ∩ same_loc)^? ⨾ ⦗W⦘ ⨾ (rf ⨾ rmw)＊) ⊆
-     ⦗set_compl C⦘ ⨾ (⦗Rel⦘ ⨾ (⦗F⦘ ⨾ sb)^? ⨾ ⦗W⦘ ⨾
-       (sb ∩ same_loc)^? ⨾ ⦗W⦘ ⨾ ⦗ set_compl I ⦘ ⨾ (⦗ set_compl I ⦘ ⨾ rf ⨾ rmw)＊)).
-  { intros x y HH.
-    destruct_seq_l HH as NC.
-    do 4 apply seqA in HH. destruct HH as [v [HH SUF]].
-    apply seq_eqv_l. split; auto.
-    
-    Ltac _ltt :=
-      apply seqA;
-      apply seqA with (r1 := ⦗Rel⦘ ⨾ (⦗F⦘ ⨾ sb)^?);
-      apply seqA with (r1 := (⦗Rel⦘ ⨾ (⦗F⦘ ⨾ sb)^?) ⨾ ⦗W⦘);
-      apply seqA with (r1 := ((⦗Rel⦘ ⨾ (⦗F⦘ ⨾ sb)^?) ⨾ ⦗W⦘) ⨾ (sb ∩ same_loc)^?).
-    
-    _ltt.
-    exists v. split.
-    { generalize HH. basic_solver. }
-    assert (release x v) as REL.
-    { unfold imm_s_hb.release, rs. _ltt.
-      eexists. split; eauto. apply rt_refl. }
-    apply seq_eqv_l. split.
-    { intros II. apply NC. eapply dom_release_issued; eauto.
-      eexists. apply seq_eqv_r. split; eauto. }
-    assert (codom_rel (⦗ set_compl C ⦘ ⨾ release) v) as XX.
-    { exists x. apply seq_eqv_l. split; auto. }
-    assert (~ I v) as NI.
-    { intros II. apply NC. eapply dom_release_issued; eauto.
-      eexists. apply seq_eqv_r. split; eauto. }
-    clear x NC HH REL.
-    induction SUF.
-    2: by apply rt_refl.
-    { apply rt_step. apply seq_eqv_l. split; auto. }
-    eapply rt_trans.
-    { by apply IHSUF1. }
-    assert (codom_rel (⦗set_compl C⦘ ⨾ release) y) as YY.
-    { destruct XX as [v XX]. destruct_seq_l XX as CC.
-      eexists. apply seq_eqv_l. split; eauto.
-      apply release_rf_rmw_steps.
-      eexists. split; eauto. }
-    apply IHSUF2; auto.
-    intros II.
-    destruct YY as [v YY]. destruct_seq_l YY as CC. apply CC.
-    eapply dom_release_issued; eauto.
-    eexists. apply seq_eqv_r. split; eauto. }
-  arewrite ((⦗set_compl I⦘ ⨾ rf ⨾ rmw)＊ ⨾
-             ⦗set_compl I⦘ ⨾ rfi ⨾ ⦗Acq⦘ ⨾ ⦗dom_rel (sb^? ⨾ ⦗I⦘)⦘ ⊆
-            sb^? ⨾ ⦗set_compl I⦘ ⨾ rfi ⨾ ⦗Acq⦘ ⨾ ⦗dom_rel (sb^? ⨾ ⦗I⦘)⦘).
-  2: { unfold Execution.rfi.
-       generalize (@sb_trans G). basic_solver. }
-  intros x y [v [HH XX]].
-  eexists. split; [|by eauto].
-  assert (dom_rel (sb ⨾ ⦗ I ⦘) v) as VV.
-  { generalize XX (@sb_trans G). unfold Execution.rfi. basic_solver 40. }
-  clear y XX.
-  induction HH as [x y HH| | ].
-  2: by apply r_refl.
-  { apply r_step.
-    destruct_seq_l HH as NIX. destruct HH as [v [RF RMW]].
-    apply rfi_union_rfe in RF. destruct RF as [RF|RF].
-    { by eapply (@sb_trans G); [apply RF|apply rmw_in_sb]. }
-    exfalso.
-    destruct VV as [z VV]. destruct_seq_r VV as AZ.
-    set (IZ := AZ).
-    apply TCCOH in IZ.
-    apply NIX. apply IZ.
-    eexists.
-    apply seq_eqv_r. split; eauto.
-    apply seq_eqv_l. split; eauto.
-    { apply (dom_l WF.(wf_rfeD)) in RF. apply seq_eqv_l in RF. desf. }
-    eapply clos_trans_mori.
-    2: apply rfe_ppo_in_ar_ct; auto.
-    { basic_solver. }
-    eexists. split; eauto.
-    red. apply seq_eqv_l. split; eauto.
-    { apply (dom_r WF.(wf_rfeD)) in RF. apply seq_eqv_r in RF. desf. }
-    apply seq_eqv_r. split; eauto.
-    2: { eapply issuedW; eauto. }
-    apply ct_step. left; right.
-    apply seq_eqv_l. split; auto.
-    { apply (dom_l WF.(wf_rmwD)) in RMW. apply seq_eqv_l in RMW. desf. }
-    eapply sb_trans; eauto. by apply rmw_in_sb. }
-  specialize (IHHH2 VV).
-  eapply (transitive_cr (@sb_trans G) _ IHHH2); eauto.
-
-  Unshelve.
-  apply IHHH1. generalize VV (@sb_trans G) IHHH2. basic_solver 10.
+  rewrite <- !seqA. rewrite dom_rel_eqv_dom_rel. rewrite !seqA.
+  arewrite (⦗FR ∩₁ Acq⦘ ⨾ sb^? ⊆ (rfe ∪ ar_int G)^?).
+  { rewrite !crE, !seq_union_r. apply union_mori; [basic_solver|].
+    unionR right. rewrite set_inter_union_l, id_union, seq_union_l.
+    rewrite sb_from_r_acq_in_bob.
+    arewrite (Acq ⊆₁ Acq/Rel) by mode_solver.
+    rewrite sb_from_f_in_bob. rewrite bob_in_ar_int. eauto with hahn. }
+  seq_rewrite ct_cr.
+  arewrite (rfe ∪ ar_int G ⊆ ar). by apply ar_ct_I_in_I.
 Qed.
 
 Lemma hb_in_Chb_sb :
   hb ⨾ ⦗C ∪₁ dom_rel (sb^? ⨾ ⦗ I ⦘)⦘ ⊆ ⦗ C ⦘ ⨾ hb ∪ sb.
-Proof using WF TCCOH RELCOV.
+Proof using WF TCCOH RELCOV IMMCON.
   unfold imm_s_hb.hb.
   intros x y HH.
   destruct_seq_r HH as DOM.
